backend/Constpropproof.v
@@ -33,7 +33,7 @@ Require Import ConstpropOpproof.
 Section PRESERVATION.
 
 Require Import ExtFunImpl ExtCallImpl.
-Existing Instances ef_ops ef_spec ec_ops ec_spec.
+Existing Instances ef_ops sc_ops ef_spec ec_ops cc_ops ec_spec.
 Context `{Hmem: Mem.MemoryModel}.
 Variable prog: program.
 Let tprog := transf_program prog.
