cfrontend/Cminorgenproof.v
@@ -38,7 +38,7 @@ Section TRANSLATION.
 
 Context `{Hmem: Mem.MemoryModel}.
 Require Import ExtFunImpl ExtCallImpl.
-Existing Instances ef_ops ef_spec ec_ops ec_spec.
+Existing Instances ef_ops sc_ops ef_spec ec_ops cc_ops ec_spec.
 
 Variable prog: Csharpminor.program.
 Variable tprog: program.
