cfrontend/Cshmgenproof.v
@@ -32,7 +32,7 @@ Require Import Cshmgen.
 
 Section WITHMEM.
 Require Import ExtFunImpl ExtCallImpl.
-Existing Instances ef_ops ef_spec ec_ops ec_spec.
+Existing Instances ef_ops sc_ops ef_spec ec_ops cc_ops ec_spec.
 Context `{Hmem: Mem.MemoryModel}.
 
 (** * Properties of operations over types *)
