cfrontend/SimplExprproof.v
@@ -34,7 +34,7 @@ Require Import SimplExprspec.
 Section PRESERVATION.
 
 Require Import ExtFunImpl ExtCallImpl.
-Existing Instances ef_ops ef_spec ec_ops ec_spec.
+Existing Instances ef_ops sc_ops ef_spec ec_ops cc_ops ec_spec.
 Context `{Hmem: Mem.MemoryModel}.
 Variable prog: Csyntax.program.
 Variable tprog: Clight.program.
