cfrontend/SimplExprspec.v
@@ -29,7 +29,7 @@ Section SPEC.
 
 Local Open Scope gensym_monad_scope.
 Require Import ExtFunImpl.
-Existing Instances ef_ops ef_spec.
+Existing Instances ef_ops sc_ops ef_spec.
 Context `{Hmem: Mem.MemoryModel}.
 
 (** * Relational specification of the translation. *)
